Examples/Simple.lean
@@ -1,0 +1,10 @@
+import Lithe
+
+open TensorExpr Tensor
+
+namespace Simple
+
+def basic : IO Unit := do
+  IO.println "Hello"
+
+end Simple
